\documentclass{beamer}
\newcommand{\myfont}{\rmfamily\normalsize\upshape\mdseries}
\newcommand{\degree}{^\circ}
\title{\sffamily Review VI(Slides 312 - 351)}
\subtitle{\textbf{Modular Arithmetic}\\}
\institute[UM-SJTU JI]{University of Michigan-Shanghai Jiao Tong University Joint Institute}
\author{HamHam}
\usepackage{graphicx}
\usepackage{picinpar}
\usepackage{indentfirst}
\usepackage{chemformula}
\usepackage{geometry}
\usepackage{subfigure}
\usepackage{appendix}
\usepackage{amsfonts}
\usepackage{enumerate}
\usepackage{float}
\usepackage{geometry}
\usepackage{latexsym}
\usepackage{listings}
\usepackage{multicol,multirow,multido}
\usepackage{tabularx}
\usepackage{ulem}
\usepackage{tikz}
\usepackage{xcolor}
\usepackage{cite}
\usepackage{setspace}
\usepackage{hyperref}
\usepackage{textpos}
\usepackage{booktabs}
\usepackage{diagbox}
\usepackage{listings}
\usepackage{graphics}
\usepackage{upgreek}
\usepackage{JI_MathCourse_Notations}
\usepackage{mathrsfs}
\usepackage[OT2,OT1]{fontenc}
%\input{../../List_of_Notation/JI_MathCourse_Notations.sty}

%\usepackage{ctex} %插入中文
%\ctexset{today=old}

\newcommand{\mydef}[1]{\sffamily\blue{#1}\myfont\\} %for define
\newcommand{\mysol}{\yellow{Solution:}\\}
\usetheme[dove]{Boadilla}
\usecolortheme{dolphin}
\useoutertheme{miniframes}
\begin{document}
    \usebackgroundtemplate{\tikz\node[opacity=0.25]{
    \includegraphics[width=\paperwidth,
    height=\paperheight]{hamster.jpg}
    };}
\begin{titlepage}
    \begin{center}
        VE203 - Discrete Mathmatics 
    \end{center}
\end{titlepage}
\myfont
\newcommand{\green}[1]{\textcolor[rgb]{0.3,0.6,0}{#1}}
\section{Modular Arithmetic}
\begin{frame}
    \frametitle{Modular Arithmetic}
    \mydef{Definition}
    \hh For $a,b\in \bZ$, and $m\in\bN\cut\{0\}$
    we say that $a$ 
    \textbf{\textit{\green{ is congruent to $b$ modulo $m$}}}, 
    writing 
    $$
        a \equiv b \mod{m}~~~~ \text{if\mbox{f}}~~~~ 
        m \mid (a-b)
    $$
    The followings are equivalent:
    \begin{itemize}
        \item $a \equiv b \mod{m}$
        \item $\underset{k\in\bZ}{\exists}\, a=b+km$
        \item $a \operatorname{mod} m = b \operatorname{mod} m$
    \end{itemize}
    \par \hh 
    For any $n \in \bZ$
    $\equiv$ is an equivalence relation on $\bZ$. 
    We call such equivalence classes 
    \textbf{congruence classes}, denoted as 
    $a := [a]_\equiv$ for $a \in \bZ$. The set of congruence classes is 
    denoted as $\bZ/n\bZ$ in consistence with the notation in group theory.
\end{frame}
\begin{frame}
    \frametitle{Modular Arithmetic}
    \hh Under a given modulo, the congruence map $a \to \bar{a}$ preserves the
    arithmetic of integers, that is
    \begin{itemize}
        \item $\conj{a+b}=\conj{a}+\conj{b}$
        \item $\conj{ab}=\conj{a}\cdot\conj{b}$
    \end{itemize}
    Or you may prefer to write:
    \begin{itemize}
        \item $a+b \equiv (a \operatorname{mod} m + b \operatorname{mod} m) \mod{m}$
        \item $a\cdot b \equiv (a \operatorname{mod} m)\cdot ( b \operatorname{mod} m) \mod{m}$
    \end{itemize}
    Thus the following two are groups:
    \begin{itemize}
        \item $\(\bZ/n\bZ,+\)$
        \item $\(\{a\in \bZ/n\bZ : \gcd(a,n=1)\},\times\)$  
        (Sometimes $\(\bZ/n\bZ,\times\)$ or $\(\bZ/n\bZ\)^\times$ for short)
    \end{itemize}
\end{frame}
\begin{frame}
    \frametitle{Exercise}
    1. Prove that $41\mid 2^{20} -1$.
    \pause
    \\\vs{2em}
    \mysol
    \hh This is equivalent to showing that
    $$2^{20}-1 \equiv 0 \mod{41}.$$
    We note that $2^5=32\equiv -9 \mod{41}$. Then
    $$2^{20}=(2^5)^4\equiv (-9)^4 \mod{41}$$
    But $(-9)^4=81\cdot 81$ and $81\equiv -1 \mod{41}$. So 
    $$2^{20} \equiv (-1)^2\equiv 1 \mod{41}$$
\end{frame}
\begin{frame}
    \frametitle{Division in Modular Arithmetic}
    \hh We have seen the addition and multiplication in 
    modular arithemetic, what about division?\\\vv
    \mydef{Theorem}
    \hh Let $a,b,c \in \bZ$ and $m \in \bN \cut \{0\}$. Then 
    $$
        ac \equiv bc \mod{m} ~~~~\Rarrow~~~~ a\equiv b \mod {m/d}
    $$
    where $d=\gcd(c,m)$.
    \\\vv 
    \mydef {Proof}
    \hh There exist integers $r,s$ with $\gcd(r,s) = 1$ such that 
    $c = rd, m = sd$. Insert them to the equation $ac - bc=k\cdot m$.
\end{frame}
\begin{frame}
    \frametitle{Modular Inverse}
    \mydef{Definition}
    \hh Let $a\in\bZ$ and $m \in \bN \cut \{ 0,1\}$ be given
    . Then an integer $a^{-1} \in \bZ $ such that 
    $$a a^{-1} \equiv 1 \mod {m}.$$
    s said to be an \green{inverse of $a$ modulo $m$}.
    \\\vs{0.5em}
    \mydef{Theorem} 
    \hh  Let $a \in \bN \cut \{0\}$ and $m \in \bN \cut \{ 0,1\}$. 
    If gcd(a, m) = 1, an inverse of $a$ modulo $m$ exists. 
    This inverse is unique modulo $m$.
    \\ \vs{0.5em}
    \mydef{Proof}
    \begin{itemize}
        \item Existence: Bézout's Theorem 
        \item Uniqueness: Prove by contradiction
    \end{itemize}
    \begin{block}{How to find the inverse}
        \hh Solve $7x\equiv 1 \mod{31}$ $\LRarrow$ Solve $7\cdot x-t\cdot 31=1$
    \end{block}
\end{frame}
\section{Arithmetic Function}
\begin{frame}
    \frametitle{Arithmetic Function}
    \mydef{Definition}
    \hh \textbf{Arithmetic function}, any mathematical function defined for integers (sometimes positive integers only)
    and dependent upon those \red{properties of the integer itself as a number}, 
    in contrast to functions that are defined for other \red{values} 
    (real numbers, complex numbers, etc.) 
    and that involve various operations from algebra and calculus.
    \\\vs{0.5em}
    \mydef{Example}
    \begin{itemize}
        \item Euler's Totient Function $\varphi(n)$
        \item $\pi(x)$, number of primes no larger than $x$
        \item $\tau(a)$, number of positive factors of $a$
        \item $\sigma(a)$, sum of all positive factors of $a$
        \item Mobius Function 
            $\mu(a)=
                \begin{cases}
                    1,~~~~~~a=1,\\
                    (-1)^r,\text{product of $r$ different primes}\\
                    0,~~~~~~\text{divisible by a prime square}
                \end{cases} 
            $ 
    \end{itemize}
\end{frame}
\begin{frame}
    \frametitle{Multiplicative Function}
    \mydef{Definition}
    \hh A function $f : \bN \cut \{0\} \to \bN\{0\}$ is multiplicative 
    if $f \(1\) = 1$ and
    $f \(m_1m_2\) = f \(m_1\)f \(m_2\)$ for $\gcd(m_1,m_2) = 1$.
    \begin{block}{Exercise}
        Check whether the followings are multiplicative functions:
        \begin{itemize}
            \item $f(n)=n^c$, where $c$ is an arbitrary constant.
            \item $f(n)=[\text{For any integer } k>1, k^2\nmid n]$.
            \item $f(n)=c^k$, where $k$ is the number of primes that divides $n$.
            \item The product of any two multiplicative functions.
        \end{itemize}
    \end{block}
    \yellow{Answer: True;~~False;~~True;~~True.}
    \\\vs{0.5em}
    \red{\textit{Comment.} This does appear in the slides!}
\end{frame}

\begin{frame}
    \frametitle{Exercise}
    2. Let $f\(x\)$ be a multiplicative function, and the 
    standard decomposition for $a$ is $a=p_1^{\alpha_1} 
    p_2^{\alpha_2}\cdots p_k^{\alpha_k}$, 
    then 
    \begin{equation*}
        \begin{aligned}
            \sum_{d\mid a} f\(d\) &= \prod_{i=1}^k
            \(1+f\(p_i\)+f\(p_i^2\)+\cdots+f\(p_i^{\alpha_i}\)\)\\
            & = \prod_{i=1}^k \,\sum_{j=0}^{\alpha_i} f\(p_i^j\)
        \end{aligned}
    \end{equation*}
    \textit{Comment.} It is easy to see that, $f\(1\)$ must be $1$. 
\end{frame}
\begin{frame}
    \frametitle{Proof}
        \hh All the positive factor of $a$ is 
        $$ 
            p_1 ^ {\beta_1} p_2 ^ {\beta_2}\cdots p_k ^ {\beta_k},
            \beta_i = 0,1,2,\cdots,\alpha_i,i=1,2,\cdots,k
        $$
        So that 
        \begin{equation*}
            \begin{aligned}
                \sum_{d\mid a} f\(d\) 
                &= \sum_{\beta_1=0}^{\alpha_1} \sum_{\beta_2=0}^{\alpha_2} 
                \cdots \sum_{\beta_k=0}^{\alpha_k} 
                f\(p_1 ^ {\beta_1} p_2 ^ {\beta_2}\cdots p_k ^ {\beta_k}\)\\
                &= \sum_{\beta_1=0}^{\alpha_1} \sum_{\beta_2=0}^{\alpha_2} 
                \cdots \sum_{\beta_k=0}^{\alpha_k} 
                f\(p_1 ^ {\beta_1}\) f\(p_2 ^ {\beta_2}\) \cdots 
                f\(p_k ^ {\beta_k}\)\\
                &= \prod_{i=1}^k
                \(f\(p_i^0\)+f\(p_i\)+f\(p_i^2\)+\cdots+f\(p_i^{\alpha_i}\)\)
            \end{aligned}
        \end{equation*}
\end{frame}
\begin{frame}
    \frametitle{Euler's Totient Function}
    \mydef{Definition}
    \hh The \blue{Euler's Totient Function}
     counts the number of positive integers less than $n$ 
     and relatively prime to $n$, i.e.
     $$ \varphi(n)= |\{k\in\bN \mid \gcd(k,n)=1,1\leq k\leq n\}| = |\(\bZ/n\bZ\)^*| $$
    \green{Properties:}
    \begin{itemize}
        \item $\varphi(p)=p-1$
        \item $\varphi(p^k)=p^k-p^{k-1} (k\geq 1)$
        \item $\varphi(mn)=\varphi(m)\cdot \varphi(n)$, if $\gcd(m,n)=1$
        \item $\varphi(n)=\sum_{d\mid n} \varphi(d)$
        \item $\varphi(a)=\varphi\(\prod_{i=1}^k p_i^{\alpha_i}\) = \prod_{i=1}^k (p_i-1)p_i^{\alpha_i-1}$
        \item $\varphi(a)=a\(1-\frac{1}{p_1}\)\(1-\frac{1}{p_2}\)\cdots\(1-\frac{1}{p_k}\)$
    \end{itemize}
\end{frame}
\begin{frame}
    \frametitle{Exercise}
    \red{This is challenging!}\\\vv
    3. Let $S_{p,q}=\{f: \bZ/p\bZ \to \bZ/q\bZ\mid
    f \text{ is a group homomorphism}\}$. Given 
    $p,q$ primes, $p<q $, then 
    \begin{itemize}
        \item[(A)] $f\(1\)=1$ if $f \in S_{p,q}$
        \item[(B)] $f$ is an isomorphism if $f \in S_{p,q}$
        \item[(C)] $|S_{p,q}|\leq |S_{q,p}|$
        \item[(D)] $|S_{p,q}| = \varphi(q)^{\varphi(p)}$  
    \end{itemize}
    \vv
    \yellow{Answer: C}
\end{frame}
\section{The. \& App.}
\begin{frame}
    \frametitle{Euler's Theorem}
    \mydef{Theorem (Euler)}
    \hh For $m \in \bN \cut \{0\}$ and $a \in \bZ$ such that $\gcd(a, m) = 1$,
    $$a ^ {\varphi(m)}\equiv 1 \mod{m}$$
    \\\vs{0.5em}
    \mydef{Proof}
    \hh Let $G=\(\bZ/m\bZ\)^*$, then $\forall a \in G$, $a^{|G|}=1_G$.
    \\\vs{0.5em}
    \green{Remark}\\
    \hh When $m\in \bP$, this becomes \blue{Fermat's Little Theorem}.
\end{frame}
\begin{frame}
    \frametitle{Exercise}
    4. Given $a, n \in \bN$ and $a, n > 1$, show that 
    $n \mid \varphi(a^n - 1)$.\\ \vv
    \pause 
    \yellow{Solution 1:}\\
    \hh Let $m=a^n-1$, consider the multiplicative group 
    $G = \(\bZ/m\bZ\)^\times$. 
    \\ \hh 
        First we prove the order of $a$ is $n$.
        Indeed, $a^n\equiv 1\mod{m}$ and 
        $a^x \not \equiv 1 \mod{m}$ for $1<x<m$
        since $1<a^x<a^n=m$.
    \\ \hh 
        According to Lagrange's theorem, therefore 
    the order of a divides the order of $G$, 
    that is, $n \mid \varphi(a^n - 1)$.
    \\ \vv
    \yellow{Solution 2:}\\
    \hh 
    \begin{equation*}
        \left.
        \begin{aligned}
            m=a^n-1 \Rarrow a^n    &\equiv 1 \mod{m}\\
            \text{Euler} \Rarrow a^{\varphi(m)}&\equiv 1 \mod{m} 
        \end{aligned}
        \right\}
        \Rarrow n \mid \varphi(m) \text{\red{~(why?)}}
    \end{equation*}
\end{frame}
\begin{frame}
    \frametitle{Fermat's Little Theorem}
    \mydef{Theorem}
    \hh Given $a \in \bZ$ and $p \in \bP$, 
    such that $(a, p) = 1$, then
    \begin{equation*}
        \begin{aligned}
            a^{p-1}&\equiv 1\mod{p}\\
            a^p    &\equiv a\mod{p}
        \end{aligned}
    \end{equation*}
    \mydef{Proof}
    \hh Induction on $a$.\\\vs{0.5em}
    \mydef{Fermat Primality Test}
    \begin{itemize}
        \item If $2^n\not\equiv 2 \mod{n}$, then n is \red{NOT} prime.
        \item If $2^n\equiv 2\mod{n}$, then n is \red{PROBABLY} prime.
    \end{itemize}
    \begin{block}{Fast Exponentiation}
        \hh Express power in binary and play with your CASIO 991CN.
    \end{block}
\end{frame}
\begin{frame}
    \frametitle{Another Proof}
    \hh Here is another proof of \blue{Fermat's Little Theorem}. \\ 
    \hh Consider the set 
        $S=\{a,2a,\cdots, (p-1)a\}$. 
    For any $ma,na$ in S, there doesn't exist 
        $ma\equiv na \mod{p}$. \red{(Why?)} Therefore
        $$ 
            S\textrm{ mod }p=
            \{0\leqslant k\leqslant p-1|ma\equiv k (\textrm{mod }p), 
            ma\in S\}=\{1,2,\cdots ,p-1\}
        $$
    Then,
        $$a\cdot 2a \cdots (p-1)a\equiv (p-1)! (\textrm{mod }p)$$
    which implies 
        $$a^{p-1}(p-1)!\equiv (p-1)! \mod{p}$$ 
    Since $\gcd\((p-1)!, p\)=1$, we conclude $a^{p-1}\equiv 1\mod{p}$.
    \begin{block}{Exercise}
        \hh Prove \blue{Euler's Theorem} by considering  
        $$S=\{ka|\textrm{gcd}(k,n)=1, 1\leqslant k\leqslant n\}$$
    \end{block}
\end{frame}
\begin{frame}
    \frametitle{Wilson's Theorem}
    \mydef{Theorem (Wilson)}
    \hh Let $p \in \bN $ be prime. Then 
        $$ (p-1)! \equiv -1 \mod{p}.$$
    \\ \vv 
    \mydef{Proof:}
    \hh \red{Key idea: find the inverse and match in pair.} \\
    \vv
    \hh The inverse $a^{-1}$ modulo $p$ of $a$ exists and is unique
    modulo $p$,
    $$a^{-1} a\equiv 1 \mod{p}$$
    
\end{frame}
\begin{frame}
    \frametitle{Proof}
     We first show that $a = a^{-1}$
    if and only if $a = 1$ or $a = p - 1$. 
    \par \vv
    It is easily checked that
    $$
        1 \cdot 1 \equiv 1 \quad\mod{p} \quad \text { and } \quad(p-1)^{2} \equiv 1 \quad\mod{p}
    $$
    Now suppose that $a^{2} \equiv 1(\bmod p)$. Then
    $$
        (a-1)(a+1) \equiv 0 \quad\mod{p}
    $$
    Since $p$ is prime, this implies $a-1 \equiv 0$ or $a+1 \equiv 0\mod{p}$. 
    Hence, either $a=1$ or $a=p-1$.
\end{frame}
\begin{frame}
    \frametitle{Proof (Cont.)}
    Next, consider the remaining $p-3$ integers
    $$
        2,3, \ldots, p-2
    $$
    Since the inverse $a^{-1}$ of $a$ is unique, 
    it follows that these numbers can be grouped 
    into pairs $a, a^{-1}$ where $a^{-1} \neq a$ and $a^{-1} a \equiv 1\mod{p}$.
    Therefore,
    $$
        (p-2) !=2 \cdot 3 \cdots(p-2) \equiv 1 \quad\mod{p}
    $$
    Multiplying by $p-1$,
    $$
        (p-1) ! \equiv p-1 \equiv-1 \quad\mod{p}
    $$
    which is what we wanted to show.
\end{frame}
\begin{frame}
    \frametitle{Chinese Remainder Theorem}
    This is from Xue Runze.\\
    \mydef{Lemma}
    \hh For $\operatorname{gcd}(m, n)=1$, we have
    $\(\bZ / m n \mathbb{Z}\) \cong \(\mathbb{Z} / m \mathbb{Z}\) \times \(\mathbb{Z} / n \mathbb{Z}\)$
    \\\vv
    \mydef{Theorem (Chinese Remainder Theorem)}
    \hh For $\operatorname{gcd}\left(m_{i}, m_{j}\right)=1$ for all $i \neq j$, we have
    $$
        \mathbb{Z} /\left(\prod_{i=1}^{n} m_{i}\right) \mathbb{Z} \cong \prod_{i=1}^{n} \mathbb{Z} / m_{i} \mathbb{Z}
    $$
    and
    $$
        \left(\mathbb{Z} /\left(\prod_{i=1}^{n} m_{i}\right) \mathbb{Z}\right)^{\times} \cong \prod_{i=1}^{n}\left(\mathbb{Z} / m_{i} \mathbb{Z}\right)^{\times}
    $$
\end{frame}
\begin{frame}
    \frametitle{Exercise}
    \green{It's better to do an exercise and make
    friends with CASIO 991CN.}\\ \vv
    5. Solve the following system of 
    \blue{linear Diophantine equations},
    $$ 
        x \equiv 3 \mod{8}, \quad 
        x \equiv 1 \mod{15}, \quad 
        x \equiv 11 \mod{20} 
    $$
   
    \textit{Comment.} Please note that $\{m_i\}^r_{i=1}$
    should be  \textbf{pairwise coprime} before 
    you apply the formula.
    \begin{block}{Recipe}
        $$
            x \equiv \sum_{i=1}^r a_i y_i \mod{m}
        $$
        where $m=\prod_{i=1}^{r} m_{i} \text { and } 
        y_{i}=\left(m / m_{i}\right)^{\varphi\left(m_{i}\right)}
         \equiv \delta_{i j} \mod{m_j}$.
    \end{block}
\end{frame}
\begin{frame}
    \frametitle{RSA Cryptography}
    For your better preparation for the exam, we here omit the technical details 
    and gives the operation steps only.\\\vv
    \begin{itemize}
        \item The \textbf{public key} to be published is a pair of positive integers 
        $(n:=p q, E)$ where $p, q \in \mathbb{P}$ and 
        $p \neq q$, and $E<\varphi(n)$, $\operatorname{gcd}(E, \varphi(n))$.
        \item The \textbf{encryption function} is
        $$
        y=e(x):=x^{E} \quad \mod{n}
        $$
        \item The private key $D:=E^{-1} \bmod \varphi(n)$. 
        The \textbf{decryption function} is therefore
        $$
        d(y):=y^{D}=x^{E D}=x \quad\mod{n}
        $$
        \item Be careful and play with CASIO 991CN.
    \end{itemize}
\end{frame}
\section{*Extra Topic}
\begin{frame}
    \frametitle{Distribution of Primes (Part II)}
    Last time we proved two lemmas:\\
    \mydef{Lemma 1}
    \hh Let $n$ be any positive integer, set
    $$N=\frac{(2n)!}{\(n!\)^2}$$  
    then 
    $$\(\pi(2n)-\pi(n)\)\ln n \leq \ln N \leq \pi(2n) \ln(2n).$$
    \mydef{Lemma 2}
    \hh For the same $n, N $ defined in Lemma 1, we have
    $$
        n \ln 2 \leq \ln N \leq 2n \ln 2.
    $$
\end{frame}
\begin{frame}
    \frametitle{Distribution of Primes (Part II)}
    Now, it's time to prove the inequality.\\
    \vv
    \mydef{Proposition}
    \hh Let $x\geq 2$, then
    $$ 0.2 \frac{x}{\ln x} \leq \pi(x) \leq 5 \frac{x}{\ln x}$$
    \mydef{Proof: (Left)}
    \hh If $x\geq 6$, let $n= \floor{x/2}$, then $x\geq 2n, n > x/3$. 
    From Lemma 1,2 we immediately obtain that 
    $$
        \pi(x)\ln x\geq \pi (2n)\ln(2n) \geq 
        \ln N \geq n \ln 2 > \frac{\ln 2 }{3}\cdot x > 0.2x
    $$
    Considering that the maximum of $x/\ln x$ on the interval 
    $[2,6]$ is $6/\ln 6$, so when $2\leq x \leq 6$,
    $$
        0.2 \frac{x}{\ln x}\leq 0.2 \frac{6}{\ln 6} <1
        = \pi(2) \leq \pi(x).
    $$
\end{frame}
\begin{frame}
    \frametitle{Proof (Right)}
    \hh From Lemma 1,2, we know
    $$
        \(\pi(2n)-\pi(n)\)\ln (n) \leq \ln N \leq 2n \ln2.
    $$
    Plug in $n=2^r$,
    $$ r \(\pi\(2^{r+1}\)-\pi\(2^r\)\) \leq 2^{r+1}.$$
    Since $\pi (2^{r+1})\leq 2^r$,
    $$
        (r+1)\pi\(2^{r+1}\)-r\pi\(2^r\) \leq 2^{r+1} + 
        \pi\(2^{r+1}\) \leq 3 \cdot 2^r
    $$
    \hh For any positive integer $m$, let $r=0,1,\cdots,m-1$, we can
    obtain $m$ inequalities.
\end{frame}
%\renewcommand{\[}{\left[}
%\renewcommand{\]}{\right]}
\begin{frame}
    \frametitle{Proof (Right)}
    \hh Add the above $m$ inequalities together,
    $$
        m \pi\(2^m\) \leq 3 (1+2+\cdots +2 ^{m-1}) < 3 \times 2^m.
    $$
    When $x\geq 2$, there exists a unique positive integer $m$
    , such that $2^{m-1} \leq x < 2 ^ m$, so $1/m < \ln 2 /\ln x$. We get 
    $$
        \pi(x) \leq \pi\(2 ^ m\) \leq \frac{1}{m}\cdot 3 \cdot 2^m\leq 
        6\ln 2 \cdot \frac{x}{\ln x }\leq 5 \frac{x}{\ln x}
    $$
    This complete out proof.\\
    \vv
    \mydef{Corollary}
    \hh Almost all the numbers are composite, namely 
    $$
        \underset{x\to \infty}{\lim} \frac{\pi(x)}{x} =0.
    $$
\end{frame}
\begin{frame}
    \frametitle{More Result}
    \mydef{Theorem}
    \hh A more advanced result, the \blue{prime number theorem}
    $$
        \underset{x\to \infty}{\lim} \frac{\pi(x)}{\frac{x}{\ln x}}=1.
    $$
    \mydef{The Best result so far}
    Let 
    $$
        li(x):=\int_2^x \frac{\mathrm{d}t}{\ln t}
    $$
    Then 
    $$
        |\pi(x) - li(x)| \leq B x e^ {-A \(\ln x \) 3/5\times (\ln \ln x)-3/5}
    $$
    \mydef{A Guess}
    $$
        |\pi(x)-li(x)| \leq B x^ {\frac{1}{2}+\varepsilon}
    $$
\end{frame}
\begin{frame}
    \frametitle{Exercise}
    6. Let $p_n$ be the n-th prime. Prove that: there exists two 
    positive numbers $B_1, B_2$, such that 
    $$ B_a n \ln n \leq p_n \leq B_2 n \ln n$$
\end{frame}
\begin{frame}
    \frametitle{Reference}
    \begin{itemize}
        \item Example From Horst's Slides FA2021.
        \item Exercises from 2021-Fall-Ve203 Mid\_2 Exam.
        \item Exercises from 2019-Fall-Ve203 TA Yan Xinyu.
        \item Contents from 2021-Fall Mid\_2\_RC by Xue Runze.
        \item Yan Shijian, etc. \textit{Basic Number Theory},
        fourth edition. Beijing: Higher Education Press, 2020.5 print.
    \end{itemize}
\end{frame}
\end{document}